theories/SetModel/CwF_pi.v
@@ -1,55 +1,12 @@
 Require Import library.
-Require Import ZF_axioms.
-Require Import ZF_library.
-Require Import CwF.
-Require Import CwF_library.
+Require Import ZF_axioms ZF_library.
+Require Import HO HO_pi.
+Require Import CwF CwF_library.
 
 (* Pi types *)
 
-Definition piTy_HO (n : nat) (Γ : ZFSet) (A : ZFSet -> ZFSet) (B : ZFSet -> ZFSet -> ZFSet) : ZFSet -> ZFSet :=
-  fun γ => ⟨ setPi n (𝕌el n (A γ)) (fun a => 𝕌el n (B γ a))
-           ; ⟨ ZFone ; typeTelescope2 n Γ A B γ ⟩ ⟩.
-
 Definition piTy (n : nat) (Γ : ZFSet) (A : ZFSet) (B : ZFSet) : ZFSet :=
-  HO_to_cwfTy n Γ (piTy_HO n Γ (cwfTy_to_HO n Γ A) (cwfTy_to_HO2 n Γ A B)).
-
-Lemma piTy_HO_typing (n : nat) {Γ : ZFSet} {A : ZFSet -> ZFSet} {B : ZFSet -> ZFSet -> ZFSet}
-  (HA : ∀ γ ∈ Γ, A γ ∈ 𝕌 n) (HB : ∀ γ ∈ Γ, ∀ a ∈ 𝕌el n (A γ), B γ a ∈ 𝕌 n) :
-  ∀ γ ∈ Γ, piTy_HO n Γ A B γ ∈ 𝕌 n.
-Proof.
-  intros γ Hγ. cbn. apply setMkPair_typing.
-  - apply setPi_typing.
-    + apply 𝕌el_typing. now apply HA.
-    + intros a Ha. apply 𝕌el_typing. now apply HB. 
-  - apply setMkPair_typing.
-    + apply one_typing.
-    + now apply typeTelescope2_typing.
-Qed.
-
-Lemma el_piTy {n : nat} {Γ γ : ZFSet} {A : ZFSet -> ZFSet} {B : ZFSet -> ZFSet -> ZFSet}
-  (HA : ∀ γ ∈ Γ, A γ ∈ 𝕌 n) (HB : ∀ γ ∈ Γ, ∀ a ∈ 𝕌el n (A γ), B γ a ∈ 𝕌 n) (Hγ : γ ∈ Γ) :
-  𝕌el n (piTy_HO n Γ A B γ) ≡ setPi n (𝕌el n (A γ)) (fun a => 𝕌el n (B γ a)).
-Proof.
-  apply setPairβ1'. now apply piTy_HO_typing.
-Qed.
-
-Lemma hd_piTy {n : nat} {Γ γ : ZFSet} {A : ZFSet -> ZFSet} {B : ZFSet -> ZFSet -> ZFSet}
-  (HA : ∀ γ ∈ Γ, A γ ∈ 𝕌 n) (HB : ∀ γ ∈ Γ, ∀ a ∈ 𝕌el n (A γ), B γ a ∈ 𝕌 n) (Hγ : γ ∈ Γ) :
-  𝕌hd n (piTy_HO n Γ A B γ) ≡ ZFone.
-Proof.
-  refine (trans (fequal (setFstPair ω (𝕍 n)) _) _).
-  apply setPairβ2'. now apply piTy_HO_typing.
-  apply setPairβ1. apply one_typing. now apply typeTelescope2_typing.
-Qed.  
-
-Lemma lbl_piTy {n : nat} {Γ γ : ZFSet} {A : ZFSet -> ZFSet} {B : ZFSet -> ZFSet -> ZFSet}
-  (HA : ∀ γ ∈ Γ, A γ ∈ 𝕌 n) (HB : ∀ γ ∈ Γ, ∀ a ∈ 𝕌el n (A γ), B γ a ∈ 𝕌 n) (Hγ : γ ∈ Γ) :
-  𝕌lbl n (piTy_HO n Γ A B γ) ≡ typeTelescope2 n Γ A B γ.
-Proof.
-  refine (trans (fequal (setSndPair ω (𝕍 n)) _) _).
-  apply setPairβ2'. now apply piTy_HO_typing.
-  apply setPairβ2. apply one_typing. now apply typeTelescope2_typing.
-Qed.
+  HO_to_cwfTy n Γ (piTy_HO n (cwfTy_to_HO n Γ A) (cwfTy_to_HO2 n Γ A B)).
 
 Lemma cwfPi {n : nat} {Γ A B : ZFSet} (HA : A ∈ cwfTy n Γ) (HB : B ∈ cwfTy n (ctxExt n Γ A)) :
   piTy n Γ A B ∈ cwfTy n Γ.
@@ -60,76 +17,14 @@ Proof.
 Qed.
 
 Lemma cwfPi_to_HO {n : nat} {Γ A B : ZFSet} (HA : A ∈ cwfTy n Γ) (HB : B ∈ cwfTy n (ctxExt n Γ A)) :
-  ∀ γ ∈ Γ, cwfTy_to_HO n Γ (piTy n Γ A B) γ ≡ piTy_HO n Γ (cwfTy_to_HO n Γ A) (cwfTy_to_HO2 n Γ A B) γ.
+  ∀ γ ∈ Γ, cwfTy_to_HO n Γ (piTy n Γ A B) γ ≡ piTy_HO n (cwfTy_to_HO n Γ A) (cwfTy_to_HO2 n Γ A B) γ.
 Proof.
   intros γ Hγ. cbn. unfold piTy. apply setAppArr_HO.
-  intros γ' Hγ'. apply piTy_HO_typing. now apply cwfTy_to_HO_typing.
+  intros γ' Hγ'. apply (piTy_HO_typing n (Γ := Γ)). now apply cwfTy_to_HO_typing.
   intros γ'' Hγ'' a Ha. now apply cwfTy_to_HO2_typing. assumption. assumption.
 Qed.
 
 (* Injectivity of Pi types *)
-
-Definition dom_piTy (n : nat) (x : ZFSet) :=
-  setFstPair (𝕌 n) (𝕍 n) (𝕌lbl n x).
-
-Definition cod_piTy (n : nat) (x : ZFSet) :=
-  setSndPair (𝕌 n) (𝕍 n) (𝕌lbl n x).
-
-Lemma dom_piTy_eq {n : nat} {Γ γ : ZFSet} {A : ZFSet -> ZFSet} {B : ZFSet -> ZFSet -> ZFSet}
-  (HA : ∀ γ ∈ Γ, A γ ∈ 𝕌 n) (HB : ∀ γ ∈ Γ, ∀ a ∈ 𝕌el n (A γ), B γ a ∈ 𝕌 n) (Hγ : γ ∈ Γ) :
-  dom_piTy n (piTy_HO n Γ A B γ) ≡ A γ.
-Proof.
-  refine (trans (fequal (setFstPair (𝕌 n) (𝕍 n)) _) _).
-  now apply lbl_piTy. apply setPairβ1. now apply HA.
-  apply HO_to_cwfTy_sorting. apply 𝕌el_typing. now apply HA. now apply HB.
-Qed.
-
-Lemma cod_piTy_eq {n : nat} {Γ γ : ZFSet} {A : ZFSet -> ZFSet} {B : ZFSet -> ZFSet -> ZFSet}
-  (HA : ∀ γ ∈ Γ, A γ ∈ 𝕌 n) (HB : ∀ γ ∈ Γ, ∀ a ∈ 𝕌el n (A γ), B γ a ∈ 𝕌 n) (Hγ : γ ∈ Γ) :
-  cod_piTy n (piTy_HO n Γ A B γ) ≡ HO_to_cwfTy n (𝕌el n (A γ)) (B γ).
-Proof.
-  refine (trans (fequal (setSndPair (𝕌 n) (𝕍 n)) _) _).
-  now apply lbl_piTy. apply setPairβ2. now apply HA.
-  apply HO_to_cwfTy_sorting. apply 𝕌el_typing. now apply HA. now apply HB.
-Qed.
-
-Lemma piTy_HO_inj1 (n : nat) {Γ γ : ZFSet} {A A' : ZFSet -> ZFSet} {B B' : ZFSet -> ZFSet -> ZFSet}
-  (HA : ∀ γ ∈ Γ, A γ ∈ 𝕌 n) (HB : ∀ γ ∈ Γ, ∀ a ∈ 𝕌el n (A γ), B γ a ∈ 𝕌 n)
-  (HA' : ∀ γ ∈ Γ, A' γ ∈ 𝕌 n) (HB' : ∀ γ ∈ Γ, ∀ a ∈ 𝕌el n (A' γ), B' γ a ∈ 𝕌 n)
-  (Hγ : γ ∈ Γ) (H : piTy_HO n Γ A B γ ≡ piTy_HO n Γ A' B' γ) : A γ ≡ A' γ.
-Proof.
-  refine (trans (b := dom_piTy n (piTy_HO n Γ A B γ)) _ _).
-  { symmetry. now apply dom_piTy_eq. }
-  refine (trans (fequal (dom_piTy n) H) _). now apply dom_piTy_eq.
-Qed.
-
-Lemma piTy_HO_inj2' (n : nat) {Γ γ : ZFSet} {A A' : ZFSet -> ZFSet} {B B' : ZFSet -> ZFSet -> ZFSet}
-  (HA : ∀ γ ∈ Γ, A γ ∈ 𝕌 n) (HB : ∀ γ ∈ Γ, ∀ a ∈ 𝕌el n (A γ), B γ a ∈ 𝕌 n)
-  (HA' : ∀ γ ∈ Γ, A' γ ∈ 𝕌 n) (HB' : ∀ γ ∈ Γ, ∀ a ∈ 𝕌el n (A' γ), B' γ a ∈ 𝕌 n)
-  (Hγ : γ ∈ Γ) (H : piTy_HO n Γ A B γ ≡ piTy_HO n Γ A' B' γ) :
-  HO_to_cwfTy n (𝕌el n (A γ)) (B γ) ≡ HO_to_cwfTy n (𝕌el n (A γ)) (B' γ).
-Proof.
-  pose proof (piTy_HO_inj1 n HA HB HA' HB' Hγ H) as HAA'.
-  refine (trans (b := cod_piTy n (piTy_HO n Γ A B γ)) _ _).
-  symmetry. now apply cod_piTy_eq. refine (trans (fequal (cod_piTy n) H) _).
-  refine (transpS (fun X => _ ≡ HO_to_cwfTy n (𝕌el n X) (B' γ)) (sym HAA') _).
-  now apply cod_piTy_eq.
-Qed.
-
-Lemma piTy_HO_inj2 (n : nat) {Γ γ a : ZFSet} {A A' : ZFSet -> ZFSet} {B B' : ZFSet -> ZFSet -> ZFSet}
-  (HA : ∀ γ ∈ Γ, A γ ∈ 𝕌 n) (HB : ∀ γ ∈ Γ, ∀ a ∈ 𝕌el n (A γ), B γ a ∈ 𝕌 n)
-  (HA' : ∀ γ ∈ Γ, A' γ ∈ 𝕌 n) (HB' : ∀ γ ∈ Γ, ∀ a ∈ 𝕌el n (A' γ), B' γ a ∈ 𝕌 n)
-  (Hγ : γ ∈ Γ) (H : piTy_HO n Γ A B γ ≡ piTy_HO n Γ A' B' γ) (Ha : a ∈ 𝕌el n (A γ)) :
-  B γ a ≡ B' γ a.
-Proof.
-  pose proof (piTy_HO_inj1 n HA HB HA' HB' Hγ H) as HAA'.
-  pose proof (piTy_HO_inj2' n HA HB HA' HB' Hγ H) as HBB'.
-  refine (trans (b := setAppArr (𝕌el n (A γ)) (𝕌 n) (HO_to_cwfTy n (𝕌el n (A γ)) (B γ)) a) _ _).
-  { symmetry. apply setAppArr_HO. intros a' Ha'. now apply HB. assumption. }
-  refine (trans (fequal (fun X => setAppArr (𝕌el n (A γ)) (𝕌 n) X a) HBB') _).
-  apply setAppArr_HO. intros a' Ha'. apply HB' ; try assumption.
-  refine (transpS (fun X => a' ∈ 𝕌el n X) HAA' _). assumption. assumption.
-Qed.
 
 (* Lemma piTy_inj1' {n : nat} {Γ γ A B A' B' : ZFSet} *)
 (*   (HA : A ∈ cwfTy n Γ) (HB : B ∈ cwfTy n (ctxExt n Γ A)) *)
@@ -156,26 +51,8 @@ Qed.
 
 (* Lambda abstraction *)
 
-Definition lamTm_HO (n : nat) (Γ : ZFSet) (A : ZFSet -> ZFSet) 
-  (t : ZFSet -> ZFSet -> ZFSet) : ZFSet -> ZFSet :=
-  fun γ => relToGraph (𝕌el n (A γ)) (𝕍 n) (HO_rel (t γ)).
-
 Definition lamTm (n : nat) (Γ : ZFSet) (A : ZFSet) (t : ZFSet) : ZFSet :=
-  HO_to_cwfTm n Γ (lamTm_HO n Γ (cwfTy_to_HO n Γ A) (cwfTm_to_HO2 n Γ A t)).
-
-Lemma lamTm_HO_typing (n : nat) {Γ : ZFSet} {A : ZFSet -> ZFSet} {B : ZFSet -> ZFSet -> ZFSet}
-  {t : ZFSet -> ZFSet -> ZFSet} (HA : ∀ γ ∈ Γ, A γ ∈ 𝕌 n) (HB : ∀ γ ∈ Γ, ∀ a ∈ 𝕌el n (A γ), B γ a ∈ 𝕌 n)
-  (Ht : ∀ γ ∈ Γ, ∀ a ∈ 𝕌el n (A γ), t γ a ∈ 𝕌el n (B γ a)) :
-  ∀ γ ∈ Γ, lamTm_HO n Γ A t γ ∈ 𝕌el n (piTy_HO n Γ A B γ).
-Proof.
-  intros γ Hγ. cbn. refine (transpS (fun X => _ ∈ X) (sym (el_piTy HA HB Hγ)) _).
-  apply ZFincomp. split.
-  - apply relToGraph_typing. apply HO_rel_typing. intros a Ha.
-    eapply ZFuniv_trans. now apply Ht. apply 𝕌el_typing. now apply HB.
-  - intros a Ha. refine (transpS (fun X => X ∈ 𝕌el n (B γ a)) _ (Ht γ Hγ a Ha)).
-    refine (sym _). apply setAppArr_HO ; [ | assumption].
-    intros a' Ha'. eapply ZFuniv_trans. now apply Ht. apply 𝕌el_typing. now apply HB.
-Qed.
+  HO_to_cwfTm n Γ (lamTm_HO n (cwfTy_to_HO n Γ A) (cwfTm_to_HO2 n Γ A t)).
 
 Lemma cwfLam {n : nat} {Γ A B t : ZFSet} (HA : A ∈ cwfTy n Γ) (HB : B ∈ cwfTy n (ctxExt n Γ A))
   (Ht : t ∈ cwfTm n (ctxExt n Γ A) B) : lamTm n Γ A t ∈ cwfTm n Γ (piTy n Γ A B).
@@ -184,7 +61,7 @@ Proof.
   - apply piTy_HO_typing.
     + now apply cwfTy_to_HO_typing.
     + intros γ Hγ a Ha. now apply cwfTy_to_HO2_typing.
-  - intros γ Hγ. apply lamTm_HO_typing.
+  - intros γ Hγ. apply (lamTm_HO_typing n (Γ := Γ)).
     + now apply cwfTy_to_HO_typing.
     + intros γ' Hγ' a Ha. now apply cwfTy_to_HO2_typing.
     + intros γ' Hγ' a Ha. now apply cwfTm_to_HO2_typing.
@@ -193,15 +70,15 @@ Qed.
 
 Lemma cwfLam_to_HO {n : nat} {Γ A B t : ZFSet} (HA : A ∈ cwfTy n Γ) (HB : B ∈ cwfTy n (ctxExt n Γ A))
   (Ht : t ∈ cwfTm n (ctxExt n Γ A) B) :
-  ∀ γ ∈ Γ, cwfTm_to_HO n Γ (lamTm n Γ A t) γ ≡ lamTm_HO n Γ (cwfTy_to_HO n Γ A) (cwfTm_to_HO2 n Γ A t) γ.
+  ∀ γ ∈ Γ, cwfTm_to_HO n Γ (lamTm n Γ A t) γ ≡ lamTm_HO n (cwfTy_to_HO n Γ A) (cwfTm_to_HO2 n Γ A t) γ.
 Proof.
   intros γ Hγ. apply setAppArr_HO. 2:assumption. clear γ Hγ.
-  intros γ Hγ. eapply ZFuniv_trans. apply (lamTm_HO_typing n (B := (cwfTy_to_HO2 n Γ A B))). 
+  intros γ Hγ. eapply ZFuniv_trans. apply (lamTm_HO_typing n (Γ := Γ) (B := (cwfTy_to_HO2 n Γ A B))). 
   - intros γ' Hγ'. now apply cwfTy_to_HO_typing.
   - intros γ' Hγ' a Ha. now apply cwfTy_to_HO2_typing.
   - intros γ' Hγ' a Ha. now apply cwfTm_to_HO2_typing.
   - assumption.
-  - apply 𝕌el_typing. apply piTy_HO_typing.
+  - apply 𝕌el_typing. apply (piTy_HO_typing n (Γ := Γ)).
     + intros γ' Hγ'. now apply cwfTy_to_HO_typing.
     + intros γ' Hγ' a Ha. now apply cwfTy_to_HO2_typing.
     + assumption.
@@ -209,23 +86,8 @@ Qed.
 
 (* Application *)
 
-Definition appTm_HO (n : nat) (Γ : ZFSet) (A : ZFSet -> ZFSet) 
-  (t : ZFSet -> ZFSet) (u : ZFSet -> ZFSet) : ZFSet -> ZFSet :=
-  fun γ => setAppArr (𝕌el n (A γ)) (𝕍 n) (t γ) (u γ).
-
 Definition appTm (n : nat) (Γ : ZFSet) (A : ZFSet) (t : ZFSet) (u : ZFSet) : ZFSet :=
-  HO_to_cwfTm n Γ (appTm_HO n Γ (cwfTy_to_HO n Γ A) (cwfTm_to_HO n Γ t) (cwfTm_to_HO n Γ u)).
-
-Lemma appTm_HO_typing (n : nat) {Γ : ZFSet} {A : ZFSet -> ZFSet} {B : ZFSet -> ZFSet -> ZFSet}
-  {t u : ZFSet -> ZFSet} (HA : ∀ γ ∈ Γ, A γ ∈ 𝕌 n) (HB : ∀ γ ∈ Γ, ∀ a ∈ 𝕌el n (A γ), B γ a ∈ 𝕌 n)
-  (Ht : ∀ γ ∈ Γ, t γ ∈ 𝕌el n (piTy_HO n Γ A B γ)) (Hu : ∀ γ ∈ Γ, u γ ∈ 𝕌el n (A γ)) :
-  ∀ γ ∈ Γ, appTm_HO n Γ A t u γ ∈ 𝕌el n (B γ (u γ)).
-Proof.
-  intros γ Hγ. assert (t γ ∈ setPi n (𝕌el n (A γ)) (fun a => 𝕌el n (B γ a))) as Htγ.
-  { refine (transpS (fun X => t γ ∈ X) _ (Ht γ Hγ)). now apply el_piTy. }
-  cbn. unfold appTm_HO. apply ZFincomp in Htγ. destruct Htγ as [ _ H ].
-  apply H. now apply Hu.
-Qed.
+  HO_to_cwfTm n Γ (appTm_HO n (cwfTy_to_HO n Γ A) (cwfTm_to_HO n Γ t) (cwfTm_to_HO n Γ u)).
 
 Lemma cwfApp {n : nat} {Γ A B t u : ZFSet} (HA : A ∈ cwfTy n Γ) (HB : B ∈ cwfTy n (ctxExt n Γ A))
   (Ht : t ∈ cwfTm n Γ (piTy n Γ A B)) (Hu : u ∈ cwfTm n Γ A) :
@@ -249,16 +111,6 @@ Qed.
 
 (* Equations (β and η) *)
 
-Lemma piTy_HO_β (n : nat) {Γ : ZFSet} {A u : ZFSet -> ZFSet} {B t : ZFSet -> ZFSet -> ZFSet}
-  (HA : ∀ γ ∈ Γ, A γ ∈ 𝕌 n) (HB : ∀ γ ∈ Γ, ∀ a ∈ 𝕌el n (A γ), B γ a ∈ 𝕌 n)
-  (Ht : ∀ γ ∈ Γ, ∀ a ∈ 𝕌el n (A γ), t γ a ∈ 𝕌el n (B γ a)) (Hu : ∀ γ ∈ Γ, u γ ∈ 𝕌el n (A γ)) :
-  ∀ γ ∈ Γ, appTm_HO n Γ A (lamTm_HO n Γ A t) u γ ≡ t γ (u γ).
-Proof.
-  intros γ Hγ. cbn. apply setAppArr_HO.
-  - intros a Ha. eapply ZFuniv_trans. now apply Ht. apply 𝕌el_typing. now apply HB.
-  - now apply Hu.
-Qed.
-
 Lemma cwfPiβ {n : nat} {Γ A B t u : ZFSet} (HA : A ∈ cwfTy n Γ) (HB : B ∈ cwfTy n (ctxExt n Γ A))
   (Ht : t ∈ cwfTm n (ctxExt n Γ A) B) (Hu : u ∈ cwfTm n Γ A) :
   appTm n Γ A (lamTm n Γ A t) u ≡ cwfTm_reindex n (ctxExt n Γ A) t Γ (sgSub n Γ A u).
@@ -273,11 +125,11 @@ Proof.
   - intros γ Hγ. refine (trans _ (sym (cwfTm_reindex_sgSub_app HA HB Ht Hu Hγ))).
     refine (trans _ _).
     { apply setAppArr_HO_to_cwfTm. 2:assumption. intros γ' Hγ'. eapply ZFuniv_trans.
-      - clear γ Hγ. apply (appTm_HO_typing n (B := (cwfTy_to_HO2 n Γ A B))).
+      - clear γ Hγ. apply (appTm_HO_typing n (Γ := Γ) (B := (cwfTy_to_HO2 n Γ A B))).
         + intros γ Hγ. now apply cwfTy_to_HO_typing.
         + intros γ Hγ a Ha. now apply cwfTy_to_HO2_typing.
         + intros γ Hγ. refine (transpS (fun X => X ∈ _) (sym (cwfLam_to_HO HA HB Ht γ Hγ)) _).
-          apply lamTm_HO_typing ; try assumption ; clear γ Hγ.
+          apply (lamTm_HO_typing n (Γ := Γ)) ; try assumption ; clear γ Hγ.
           * intros γ Hγ. now apply cwfTy_to_HO_typing.
           * intros γ Hγ a Ha. now apply cwfTy_to_HO2_typing.
           * intros γ Hγ a Ha. now apply cwfTm_to_HO2_typing.
@@ -293,24 +145,6 @@ Proof.
         apply 𝕌el_typing. now apply cwfTy_to_HO2_typing.
       - now apply cwfTm_to_HO_typing. }
     reflexivity.
-Qed.
-
-Lemma piTy_HO_η (n : nat) {Γ : ZFSet} {A t : ZFSet -> ZFSet} {B : ZFSet -> ZFSet -> ZFSet}
-  (HA : ∀ γ ∈ Γ, A γ ∈ 𝕌 n) (HB : ∀ γ ∈ Γ, ∀ a ∈ 𝕌el n (A γ), B γ a ∈ 𝕌 n)
-  (Ht : ∀ γ ∈ Γ, t γ ∈ 𝕌el n (piTy_HO n Γ A B γ)) :
-  ∀ γ ∈ Γ, t γ ≡ lamTm_HO n Γ A (fun γ a => appTm_HO n Γ A t (fun γ => a) γ) γ.
-Proof.
-  intros γ Hγ. cbn. unfold lamTm_HO. unfold appTm_HO.
-  assert (t γ ∈ setPi n (𝕌el n (A γ)) (fun a => 𝕌el n (B γ a))) as Ht'.
-  { refine (transpS (fun X => t γ ∈ X) (el_piTy HA HB Hγ) _). now apply Ht. }
-  apply ZFincomp in Ht'. destruct Ht' as [ Ht' _ ].
-  change (fun a : ZFSet => setAppArr (𝕌el n (A γ)) (𝕍 n) (t γ) a) with (setAppArr (𝕌el n (A γ)) (𝕍 n) (t γ)).
-  apply (setArr_funext (A := 𝕌el n (A γ)) (B := 𝕍 n)).
-  - exact Ht'.
-  - apply relToGraph_typing. apply HO_rel_typing.
-    intros a Ha. apply setAppArr_typing. 2:assumption. exact Ht'.
-  - intros a Ha. refine (sym _). apply setAppArr_HO. 2:assumption. clear a Ha.
-    intros a Ha. apply setAppArr_typing. 2:assumption. exact Ht'.
 Qed.
 
 Lemma cwfPiη_aux {n : nat} {Γ A B t : ZFSet} (HA : A ∈ cwfTy n Γ)
@@ -354,11 +188,11 @@ Proof.
     apply ZFincomp in H. destruct H as [ H _ ]. exact H.
   - intros γ Hγ. refine (sym (trans _ _)).
     { apply setAppArr_HO. 2:assumption. clear γ Hγ.
-      intros γ Hγ. eapply ZFuniv_trans. apply (lamTm_HO_typing n (B := (cwfTy_to_HO2 n Γ A B))) ; try assumption ; clear γ Hγ.
+      intros γ Hγ. eapply ZFuniv_trans. apply (lamTm_HO_typing n (Γ := Γ) (B := (cwfTy_to_HO2 n Γ A B))) ; try assumption ; clear γ Hγ.
       - intros γ Hγ. now apply cwfTy_to_HO_typing.
       - intros γ Hγ a Ha. now apply cwfTy_to_HO2_typing.
       - intros γ Hγ a Ha. apply cwfTm_to_HO2_typing ; try assumption. now apply cwfPiη_aux.
-      - apply 𝕌el_typing. apply piTy_HO_typing.
+      - apply 𝕌el_typing. apply (piTy_HO_typing n (Γ := Γ)).
         + intros γ' Hγ'. now apply cwfTy_to_HO_typing.
         + intros γ' Hγ' a Ha. now apply cwfTy_to_HO2_typing.
         + assumption. }
