theories/SetModel/HO_model.v
@@ -1,0 +1,67 @@
+From Stdlib Require Import Utf8 List Arith Bool.
+From TypedConfluence Require Import core unscoped AST SubstNotations RAsimpl AST_rasimpl.
+From TypedConfluence Require Import Util BasicAST Contexts Typing BasicMetaTheory Reduction. 
+From Stdlib Require Import Setoid Morphisms Relation_Definitions.
+
+Import ListNotations.
+Import CombineNotations.
+
+Require Import library.
+Require Import ZF_axioms ZF_library.
+Require Import HO HO_pi HO_sigma HO_nat.
+
+Open Scope subst_scope.
+
+Definition to_ZF_level (l : level) : nat :=
+  match l with
+  | ty n => n
+  | prop => 0
+  end.
+
+Inductive interp_ctx : forall (Γ : ctx), ZFSet -> SProp :=
+
+| interp_empty : interp_ctx ∙ (setSingl ∅)
+
+| interp_cons  : forall Γ l A iΓ iA, interp_ctx Γ iΓ -> interp_tm Γ l A iA
+                 -> interp_ctx (Γ ,, (l , A)) (setSigma (to_ZF_level l) iΓ (fun γ => 𝕌el (to_ZF_level l) (iA γ)))
+
+with is_nth_proj : forall (Γ : ctx), (ZFSet -> ZFSet) -> SProp :=
+| here :
+  -> is_nth_proj (Γ ,, (l , A)) (fun γa => setSndSigma (to_ZF_level l) Γi (fun γ => 𝕌el (to_ZF_level l) (iA γ)) γa)
+
+with interp_tm : forall (Γ : ctx) (l : level) (A : term), (ZFSet -> ZFSet) -> SProp :=
+
+| interp_pi : forall Γ lA lB A B iΓ iA iB, interp_tm Γ lA A iA
+              -> interp_tm (Γ ,, (lA , A)) (ty lB) B iB
+              -> interp_tm Γ (Ru lA (ty lB)) (Pi lA (ty lB) A B) (piTy_HO (to_ZF_level (Ru lA (ty lB))) iΓ iA (fun γ a => iB ⟨ γ ; a ⟩))
+
+(* | interp_forall :  *)
+
+| interp_nat : forall Γ, interp_tm Γ (ty 0) Nat natTy_HO
+
+| interp_type : forall Γ l, interp_tm Γ (Ax (ty l)) (Sort (ty l)) natTy_HO
+
+| interp_prop : forall Γ l, interp_tm Γ (Ax (ty l)) (Sort (ty l)) natTy_HO
+
+(* | interp_acc : ... *)
+
+| interp_
+
+piTy_HO (n : nat) (Γ : ZFSet) (A : ZFSet -> ZFSet) (B : ZFSet -> ZFSet -> ZFSet) : ZFSet -> ZFSet :=
+
+
+
+with interp_tm : forall (Γ : ctx) (l : level) (t : term), (ZFSet -> ZFSet) -> SProp :=
+| interp_var : is_nth_proj Γ π 
+    -> interp_tm Γ l (var x) π
+
+
+
+Γ ⊢ t : A
+
+∀ γ ∈ ⟦ Γ ⟧, ⟦ Γ ⊢ t ⟧γ ∈ ⟦ Γ ⊢ A ⟧γ
+
+Lemma model : forall Γ l t A, Γ ⊢< l > t : A -> True.
+
+(forall Γ l t A, Γ ⊢< l > t : A -> forall k (_temp : l = ty k), Γ ⊢< l > t ≡ t : A -> Γ ⊨< l > t ≡ t : A) ∧
+      (forall Γ l t u A, Γ ⊢< l > t ≡ u : A -> forall k (_temp : l = ty k), Γ ⊢< l > t ≡ u : A -> Γ ⊨< l > t ≡ u : A).
