theories/SetModel/HO_nat.v
@@ -1,0 +1,64 @@
+Require Import library.
+Require Import ZF_axioms ZF_library.
+Require Import HO HO_pi.
+
+Definition natTy_HO : ZFSet -> ZFSet := fun _ => ⟨ ω ; ⟨ ∅ ; ∅ ⟩ ⟩.
+
+Lemma el_natTy {n : nat} {γ : ZFSet} : 𝕌el n (natTy_HO γ) ≡ ω.
+Proof.
+  apply setPairβ1.
+  + apply ZFuniv_uncountable.
+  + apply setMkPair_typing. apply zero_typing. apply empty_in_univ.
+Qed.
+
+Lemma natTy_HO_typing (n : nat) {γ : ZFSet} : natTy_HO γ ∈ 𝕌 n.
+Proof.
+  apply setMkPair_typing.
+  - now apply ZFuniv_uncountable.
+  - apply setMkPair_typing.
+    + apply zero_typing.
+    + apply empty_in_univ.
+Qed.
+
+(* Zero *)
+
+Definition zeroTm_HO : ZFSet -> ZFSet := fun _ => ∅.
+
+Lemma zeroTm_HO_typing (n : nat) {γ : ZFSet} : zeroTm_HO γ ∈ 𝕌el n (natTy_HO γ).
+Proof.
+  refine (transpS (fun x => _ ∈ x) _ _).
+  - symmetry. apply el_natTy. 
+  - apply zero_typing.
+Qed.
+
+(* Successor *)
+
+Definition sucTm_HO (n : nat) (t : ZFSet -> ZFSet) : ZFSet -> ZFSet :=
+  fun γ => ZFsuc (t γ).
+
+Lemma sucTm_HO_typing {n : nat} {Γ γ : ZFSet} {t : ZFSet -> ZFSet} (Ht : ∀ γ ∈ Γ, t γ ∈ 𝕌el n (natTy_HO γ)) (Hγ : γ ∈ Γ) :
+  sucTm_HO n t γ ∈ 𝕌el n (natTy_HO γ).
+Proof.
+  refine (transpS (fun x => _ ∈ x) _ _).
+  { symmetry. apply el_natTy. }
+  apply suc_typing.
+  refine (transpS (fun x => _ ∈ x) _ _).
+  { apply (@el_natTy n γ). }
+  now apply Ht.
+Qed.
+
+(* Recursor *)
+
+Definition natrecTm_HO (n : nat) (P : ZFSet -> ZFSet -> ZFSet) (pz : ZFSet -> ZFSet)
+  (ps : ZFSet -> ZFSet -> ZFSet -> ZFSet) (m : ZFSet -> ZFSet) : ZFSet -> ZFSet :=
+  fun γ => natrec2 n (P γ) (pz γ) (ps γ) (m γ).
+
+(* Lemma natrecTm_HO_typing {n : nat} {Γ : ZFSet} {P : ZFSet -> ZFSet -> ZFSet} {pz : ZFSet -> ZFSet} *)
+(*   {ps : ZFSet -> ZFSet -> ZFSet -> ZFSet} {m : ZFSet -> ZFSet} *)
+(*   (HP : ∀ γ ∈ Γ, ∀ m ∈ 𝕌el n (natTy_HO γ), P γ m ∈ 𝕌 n) (Hpz : ∀ γ ∈ Γ, pz Γ ∈ P γ (zeroTm_HO γ)) *)
+(*   (Hps : ∀ γ ∈ Γ, ∀ m ∈ 𝕌el n (natTy_HO γ), ∀ pm ∈ 𝕌el n (P γ m), *)
+(*       ps γ m pm ∈ P γ (sucTm_HO n (fun γnp => ))) *)
+(*   (Hm : ∀ γ ∈ Γ, m γ ∈ 𝕌el n (natTy_HO γ)) :  *)
+(*   ∀ γ ∈ Γ, natrecTm_HO n P pz ps m ∈ 𝕌el n (P γ m). *)
+
+(* Definition sucTm_HO (n : nat) (t : ZFSet -> ZFSet) : ZFSet -> ZFSet := *)
