theories/SetModel/HO_sigma.v
@@ -1,0 +1,192 @@
+Require Import library.
+Require Import ZF_axioms ZF_library.
+Require Import HO.
+
+(* Sigma types *)
+
+Definition sigmaTy_HO (n : nat) (A : ZFSet -> ZFSet) (B : ZFSet -> ZFSet -> ZFSet) : ZFSet -> ZFSet :=
+  fun γ => ⟨ setSigma n (𝕌el n (A γ)) (fun a => 𝕌el n (B γ a))
+           ; ⟨ ZFtwo ; typeTelescope2 n A B γ ⟩ ⟩.
+
+Lemma sigmaTy_HO_typing (n : nat) {Γ : ZFSet} {A : ZFSet -> ZFSet} {B : ZFSet -> ZFSet -> ZFSet}
+  (HA : ∀ γ ∈ Γ, A γ ∈ 𝕌 n) (HB : ∀ γ ∈ Γ, ∀ a ∈ 𝕌el n (A γ), B γ a ∈ 𝕌 n) :
+  ∀ γ ∈ Γ, sigmaTy_HO n A B γ ∈ 𝕌 n.
+Proof.
+  intros γ Hγ. cbn. apply setMkPair_typing.
+  - apply setSigma_typing.
+    + apply 𝕌el_typing. now apply HA.
+    + intros a Ha. apply 𝕌el_typing. now apply HB. 
+  - apply setMkPair_typing.
+    + apply two_typing.
+    + now apply (typeTelescope2_typing n (Γ := Γ)).
+Qed.
+
+Lemma el_sigmaTy {n : nat} {Γ γ : ZFSet} {A : ZFSet -> ZFSet} {B : ZFSet -> ZFSet -> ZFSet}
+  (HA : ∀ γ ∈ Γ, A γ ∈ 𝕌 n) (HB : ∀ γ ∈ Γ, ∀ a ∈ 𝕌el n (A γ), B γ a ∈ 𝕌 n) (Hγ : γ ∈ Γ) :
+  𝕌el n (sigmaTy_HO n A B γ) ≡ setSigma n (𝕌el n (A γ)) (fun a => 𝕌el n (B γ a)).
+Proof.
+  apply setPairβ1'. now apply (sigmaTy_HO_typing n (Γ := Γ)).
+Qed.
+
+Lemma hd_sigmaTy {n : nat} {Γ γ : ZFSet} {A : ZFSet -> ZFSet} {B : ZFSet -> ZFSet -> ZFSet}
+  (HA : ∀ γ ∈ Γ, A γ ∈ 𝕌 n) (HB : ∀ γ ∈ Γ, ∀ a ∈ 𝕌el n (A γ), B γ a ∈ 𝕌 n) (Hγ : γ ∈ Γ) :
+  𝕌hd n (sigmaTy_HO n A B γ) ≡ ZFtwo.
+Proof.
+  refine (trans (fequal (setFstPair ω (𝕍 n)) _) _).
+  apply setPairβ2'. now apply (sigmaTy_HO_typing n (Γ := Γ)).
+  apply setPairβ1. apply two_typing. now apply (typeTelescope2_typing n (Γ := Γ)).
+Qed.  
+
+Lemma lbl_sigmaTy {n : nat} {Γ γ : ZFSet} {A : ZFSet -> ZFSet} {B : ZFSet -> ZFSet -> ZFSet}
+  (HA : ∀ γ ∈ Γ, A γ ∈ 𝕌 n) (HB : ∀ γ ∈ Γ, ∀ a ∈ 𝕌el n (A γ), B γ a ∈ 𝕌 n) (Hγ : γ ∈ Γ) :
+  𝕌lbl n (sigmaTy_HO n A B γ) ≡ typeTelescope2 n A B γ.
+Proof.
+  refine (trans (fequal (setSndPair ω (𝕍 n)) _) _).
+  apply setPairβ2'. now apply (sigmaTy_HO_typing n (Γ := Γ)).
+  apply setPairβ2. apply two_typing. now apply (typeTelescope2_typing n (Γ := Γ)).
+Qed.
+
+(* Injectivity of Sigma types *)
+
+Definition dom_sigmaTy (n : nat) (x : ZFSet) :=
+  setFstPair (𝕌 n) (𝕍 n) (𝕌lbl n x).
+
+Definition cod_sigmaTy (n : nat) (x : ZFSet) :=
+  setSndPair (𝕌 n) (𝕍 n) (𝕌lbl n x).
+
+Lemma dom_sigmaTy_eq {n : nat} {Γ γ : ZFSet} {A : ZFSet -> ZFSet} {B : ZFSet -> ZFSet -> ZFSet}
+  (HA : ∀ γ ∈ Γ, A γ ∈ 𝕌 n) (HB : ∀ γ ∈ Γ, ∀ a ∈ 𝕌el n (A γ), B γ a ∈ 𝕌 n) (Hγ : γ ∈ Γ) :
+  dom_sigmaTy n (sigmaTy_HO n A B γ) ≡ A γ.
+Proof.
+  refine (trans (fequal (setFstPair (𝕌 n) (𝕍 n)) _) _).
+  now apply (lbl_sigmaTy (Γ := Γ)). apply setPairβ1. now apply HA.
+  apply typeToGraph_sorting. now apply HA. now apply HB.
+Qed.
+
+Lemma cod_sigmaTy_eq {n : nat} {Γ γ : ZFSet} {A : ZFSet -> ZFSet} {B : ZFSet -> ZFSet -> ZFSet}
+  (HA : ∀ γ ∈ Γ, A γ ∈ 𝕌 n) (HB : ∀ γ ∈ Γ, ∀ a ∈ 𝕌el n (A γ), B γ a ∈ 𝕌 n) (Hγ : γ ∈ Γ) :
+  cod_sigmaTy n (sigmaTy_HO n A B γ) ≡ typeToGraph n (A γ) (B γ).
+Proof.
+  refine (trans (fequal (setSndPair (𝕌 n) (𝕍 n)) _) _).
+  now apply (lbl_sigmaTy (Γ := Γ)). apply setPairβ2. now apply HA.
+  apply typeToGraph_sorting. now apply HA. now apply HB.
+Qed.
+
+Lemma sigmaTy_HO_inj1 (n : nat) {Γ γ : ZFSet} {A A' : ZFSet -> ZFSet} {B B' : ZFSet -> ZFSet -> ZFSet}
+  (HA : ∀ γ ∈ Γ, A γ ∈ 𝕌 n) (HB : ∀ γ ∈ Γ, ∀ a ∈ 𝕌el n (A γ), B γ a ∈ 𝕌 n)
+  (HA' : ∀ γ ∈ Γ, A' γ ∈ 𝕌 n) (HB' : ∀ γ ∈ Γ, ∀ a ∈ 𝕌el n (A' γ), B' γ a ∈ 𝕌 n)
+  (Hγ : γ ∈ Γ) (H : sigmaTy_HO n A B γ ≡ sigmaTy_HO n A' B' γ) : A γ ≡ A' γ.
+Proof.
+  refine (trans (b := dom_sigmaTy n (sigmaTy_HO n A B γ)) _ _).
+  { symmetry. now apply (dom_sigmaTy_eq (Γ := Γ)). }
+  refine (trans (fequal (dom_sigmaTy n) H) _). now apply (dom_sigmaTy_eq (Γ := Γ)).
+Qed.
+
+Lemma sigmaTy_HO_inj2' (n : nat) {Γ γ : ZFSet} {A A' : ZFSet -> ZFSet} {B B' : ZFSet -> ZFSet -> ZFSet}
+  (HA : ∀ γ ∈ Γ, A γ ∈ 𝕌 n) (HB : ∀ γ ∈ Γ, ∀ a ∈ 𝕌el n (A γ), B γ a ∈ 𝕌 n)
+  (HA' : ∀ γ ∈ Γ, A' γ ∈ 𝕌 n) (HB' : ∀ γ ∈ Γ, ∀ a ∈ 𝕌el n (A' γ), B' γ a ∈ 𝕌 n)
+  (Hγ : γ ∈ Γ) (H : sigmaTy_HO n A B γ ≡ sigmaTy_HO n A' B' γ) :
+  typeToGraph n (A γ) (B γ) ≡ typeToGraph n (A γ) (B' γ).
+Proof.
+  pose proof (sigmaTy_HO_inj1 n HA HB HA' HB' Hγ H) as HAA'.
+  refine (trans (b := cod_sigmaTy n (sigmaTy_HO n A B γ)) _ _).
+  symmetry. now apply (cod_sigmaTy_eq (Γ := Γ)). refine (trans (fequal (cod_sigmaTy n) H) _).
+  refine (transpS (fun X => _ ≡ typeToGraph n X (B' γ)) (sym HAA') _).
+  now apply (cod_sigmaTy_eq (Γ := Γ)).
+Qed.
+
+Lemma sigmaTy_HO_inj2 (n : nat) {Γ γ a : ZFSet} {A A' : ZFSet -> ZFSet} {B B' : ZFSet -> ZFSet -> ZFSet}
+  (HA : ∀ γ ∈ Γ, A γ ∈ 𝕌 n) (HB : ∀ γ ∈ Γ, ∀ a ∈ 𝕌el n (A γ), B γ a ∈ 𝕌 n)
+  (HA' : ∀ γ ∈ Γ, A' γ ∈ 𝕌 n) (HB' : ∀ γ ∈ Γ, ∀ a ∈ 𝕌el n (A' γ), B' γ a ∈ 𝕌 n)
+  (Hγ : γ ∈ Γ) (H : sigmaTy_HO n A B γ ≡ sigmaTy_HO n A' B' γ) (Ha : a ∈ 𝕌el n (A γ)) :
+  B γ a ≡ B' γ a.
+Proof.
+  pose proof (sigmaTy_HO_inj1 n HA HB HA' HB' Hγ H) as HAA'.
+  pose proof (sigmaTy_HO_inj2' n HA HB HA' HB' Hγ H) as HBB'.
+  refine (trans (b := setAppArr (𝕌el n (A γ)) (𝕌 n) (typeToGraph n (A γ) (B γ)) a) _ _).
+  { symmetry. apply setAppArr_HO. intros a' Ha'. now apply HB. assumption. }
+  refine (trans (fequal (fun X => setAppArr (𝕌el n (A γ)) (𝕌 n) X a) HBB') _).
+  apply setAppArr_HO. intros a' Ha'. apply HB' ; try assumption.
+  refine (transpS (fun X => a' ∈ 𝕌el n X) HAA' _). assumption. assumption.
+Qed.
+
+(* Pairing *)
+
+Definition pairTm_HO (n : nat) (t : ZFSet -> ZFSet) (u : ZFSet -> ZFSet) : ZFSet -> ZFSet :=
+  fun γ => ⟨ t γ ; u γ ⟩.
+
+Lemma pairTm_HO_typing {n : nat} {Γ : ZFSet} {A t u : ZFSet -> ZFSet} {B : ZFSet -> ZFSet -> ZFSet}
+  (HA : ∀ γ ∈ Γ, A γ ∈ 𝕌 n) (HB : ∀ γ ∈ Γ, ∀ a ∈ 𝕌el n (A γ), B γ a ∈ 𝕌 n)
+  (Ht : ∀ γ ∈ Γ, t γ ∈ 𝕌el n (A γ)) (Hu : ∀ γ ∈ Γ, u γ ∈ 𝕌el n (B γ (t γ)))
+  : ∀ γ ∈ Γ, pairTm_HO n t u γ ∈ 𝕌el n (sigmaTy_HO n A B γ).
+Proof.
+  intros γ Hγ. cbn. refine (transpS (fun X => _ ∈ X) (sym (el_sigmaTy HA HB Hγ)) _). apply setMkSigma_typing.
+  - intros a Ha. apply 𝕌el_typing. now apply HB.
+  - now apply Ht.
+  - now apply Hu.
+Qed.
+
+(* First projection *)
+
+Definition fstTm_HO (n : nat) (A : ZFSet -> ZFSet)
+  (B : ZFSet -> ZFSet -> ZFSet) (t : ZFSet -> ZFSet) : ZFSet -> ZFSet :=
+  fun γ => setFstSigma n (𝕌el n (A γ)) (fun a => 𝕌el n (B γ a)) (t γ).
+
+Lemma fstTm_HO_typing {n : nat} {Γ : ZFSet} {A t : ZFSet -> ZFSet} {B : ZFSet -> ZFSet -> ZFSet}
+  (HA : ∀ γ ∈ Γ, A γ ∈ 𝕌 n) (HB : ∀ γ ∈ Γ, ∀ a ∈ 𝕌el n (A γ), B γ a ∈ 𝕌 n)
+  (Ht : ∀ γ ∈ Γ, t γ ∈ 𝕌el n (sigmaTy_HO n A B γ)) : ∀ γ ∈ Γ, fstTm_HO n A B t γ ∈ 𝕌el n (A γ).
+Proof.
+  intros γ Hγ. cbn. unfold fstTm_HO. apply setFstSigma_typing.
+  - intros a Ha. apply 𝕌el_typing. now apply HB.
+  - refine (transpS (fun X => _ ∈ X) (el_sigmaTy HA HB Hγ) _). now apply Ht.
+Qed.
+
+(* Second projection *)
+
+Definition sndTm_HO (n : nat) (A : ZFSet -> ZFSet)
+  (B : ZFSet -> ZFSet -> ZFSet) (t : ZFSet -> ZFSet) : ZFSet -> ZFSet :=
+  fun γ => setSndSigma n (𝕌el n (A γ)) (fun a => 𝕌el n (B γ a)) (t γ).
+
+Lemma sndTm_HO_typing {n : nat} {Γ : ZFSet} {A t : ZFSet -> ZFSet} {B : ZFSet -> ZFSet -> ZFSet}
+  (HA : ∀ γ ∈ Γ, A γ ∈ 𝕌 n) (HB : ∀ γ ∈ Γ, ∀ a ∈ 𝕌el n (A γ), B γ a ∈ 𝕌 n)
+  (Ht : ∀ γ ∈ Γ, t γ ∈ 𝕌el n (sigmaTy_HO n A B γ)) : ∀ γ ∈ Γ, sndTm_HO n A B t γ ∈ 𝕌el n (B γ (fstTm_HO n A B t γ)).
+Proof.
+  intros γ Hγ. cbn. unfold fstTm_HO. refine (transpS (fun X => _ ∈ X) _ _).
+  2:{ apply setSndSigma_typing.
+      - intros a Ha. apply 𝕌el_typing. now apply HB.
+      - refine (transpS (fun X => _ ∈ X) (el_sigmaTy HA HB Hγ) _). now apply Ht. }
+  reflexivity.
+Qed.
+
+(* Equations (β and η) *)
+
+Lemma sigmaTy_HO_β1 {n : nat} {Γ : ZFSet} {A t u : ZFSet -> ZFSet} {B : ZFSet -> ZFSet -> ZFSet}
+  (HA : ∀ γ ∈ Γ, A γ ∈ 𝕌 n) (HB : ∀ γ ∈ Γ, ∀ a ∈ 𝕌el n (A γ), B γ a ∈ 𝕌 n)
+  (Ht : ∀ γ ∈ Γ, t γ ∈ 𝕌el n (A γ)) (Hu : ∀ γ ∈ Γ, u γ ∈ 𝕌el n (B γ (t γ))) :
+  ∀ γ ∈ Γ, fstTm_HO n A B (pairTm_HO n t u) γ ≡ t γ.
+Proof.
+  intros γ Hγ. cbn. apply setSigmaβ1.
+  - intros a Ha. apply 𝕌el_typing. now apply HB.
+  - now apply Ht.
+  - now apply Hu.
+Qed.
+
+Lemma sigmaTy_HO_β2 {n : nat} {Γ : ZFSet} {A t u : ZFSet -> ZFSet} {B : ZFSet -> ZFSet -> ZFSet}
+  (HA : ∀ γ ∈ Γ, A γ ∈ 𝕌 n) (HB : ∀ γ ∈ Γ, ∀ a ∈ 𝕌el n (A γ), B γ a ∈ 𝕌 n)
+  (Ht : ∀ γ ∈ Γ, t γ ∈ 𝕌el n (A γ)) (Hu : ∀ γ ∈ Γ, u γ ∈ 𝕌el n (B γ (t γ))) :
+  ∀ γ ∈ Γ, sndTm_HO n A B (pairTm_HO n t u) γ ≡ u γ.
+Proof.
+  intros γ Hγ. cbn. apply setSigmaβ2.
+  - intros a Ha. apply 𝕌el_typing. now apply HB.
+  - now apply Ht.
+  - now apply Hu.
+Qed.
+
+Lemma sigmaTy_HO_η {n : nat} {Γ : ZFSet} {A t : ZFSet -> ZFSet} {B : ZFSet -> ZFSet -> ZFSet}
+  (HA : ∀ γ ∈ Γ, A γ ∈ 𝕌 n) (HB : ∀ γ ∈ Γ, ∀ a ∈ 𝕌el n (A γ), B γ a ∈ 𝕌 n) (Ht : ∀ γ ∈ Γ, t γ ∈ 𝕌el n (sigmaTy_HO n A B γ)) :
+  ∀ γ ∈ Γ, t γ ≡ pairTm_HO n (fstTm_HO n A B t) (sndTm_HO n A B t) γ.
+Proof.
+  intros γ Hγ. cbn. apply setSigmaη.
+  - intros a Ha. apply 𝕌el_typing. now apply HB.
+  - refine (transpS (fun X => _ ∈ X) (el_sigmaTy HA HB Hγ) _). now apply Ht.
+Qed.
